Meta: Axiom.Union test

coq/ZF/Meta/Test/Axiom/Union.v
@@ -1,23 +1,16 @@
-Require Import ZF.Meta.Ctx.
-Require Import ZF.Meta.Env.
+Require Import Coq.Lists.List.
+Require Import Coq.Strings.String.
+
 Require Import ZF.Meta.Syntax.
 Require Import ZF.Meta.Check.
+Require Import ZF.Meta.Term.CheckDecl.
 Require Import ZF.Meta.Ty.
 
-(* forall a, exists b, forall x, x :< b <-> exists y, x :< y /\ y :< a          *)
-Definition Union : Term :=
-  All VarTySet
-    (Ex VarTySet
-      (All VarTySet
-        (Iff
-          (Elem (Var 0) (Var 1))
-          (Ex VarTySet
-            (And
-              (Elem (Var 1) (Var 0))
-              (Elem (Var 0) (Var 3))))))).
+Import ListNotations.
 
-(* The union example is a proposition in the empty environment.                 *)
-Proposition Check : CheckT Env.empty Ctx.empty Union TyProp.
+Require Import ZF.Meta.Decl.Axiom.Union.
+
+Proposition Union : CheckDeclT (Union.env) Union.
 Proof.
   (* Proof by Hermes + gpt 5.5                                                  *)
   apply CheckAll, CheckEx, CheckAll, CheckIff.
