coq/ZF/Meta/Decl/Axiom/Union.v
@@ -1,0 +1,33 @@
+Require Import Coq.Lists.List.
+Require Import Coq.Strings.String.
+
+Require Import ZF.Meta.Env.
+Require Import ZF.Meta.Syntax.
+Require Import ZF.Meta.Term.Decl.
+Require Import ZF.Meta.Ty.
+
+Import ListNotations.
+
+(* forall a, exists b, forall x, x :< b <-> exists y, x :< y /\ y :< a          *)
+Definition Union : DeclT :=
+  {| paraT := []
+  ;  resT  := TyProp
+  ;  bodyT :=
+      All VarTySet
+        (Ex VarTySet
+          (All VarTySet
+            (Iff
+              (Elem (Var 0) (Var 1))
+              (Ex VarTySet
+                (And
+                  (Elem (Var 1) (Var 0))
+                  (Elem (Var 0) (Var 3)))))))
+  |}.
+
+Definition imports : Env := Env.empty.
+
+Definition exports : Env := Env.fromListT
+  [ ("Union"%string, Union)
+  ].
+
+Definition env : Env := Env.union imports exports.
